add subst-free semantics for ElimFunc & TaggedNumbered; start on new TaggedNumbered -> ElimFunc compiler

src/ElimFuncComp.v
@@ -1,22 +1,68 @@
 Require Import Common Monads.
-Require Tagged ElimFunc.
+Require TaggedNumbered ElimFunc.
 
-Module T := Tagged.
+Require Import Psatz.
+
+Module T := TaggedNumbered.
 Module E := ElimFunc.
 
-Definition compiler_monad A := state (list E.expr) A.
 
+Fixpoint upvar_list' acc n :=
+    match n with
+    | 0 => E.Arg :: acc
+    | S n' => upvar_list' (E.UpVar n' :: acc) n'
+    end.
 
 Definition upvar_list n :=
-    let fix go acc n :=
-        match n with
-        | 0 => E.Arg :: acc
-        | S n' => go (E.UpVar n' :: acc) n'
-        end in
     match n with
     | 0 => []
-    | S n' => go [] n'
+    | S n' => upvar_list' [] n'
     end.
+
+Definition compile base :=
+    let fix go e :=
+        let fix go_list es :=
+            match es with
+            | [] => []
+            | e :: es => go e :: go_list es
+            end in
+        match e with
+        | T.Arg => E.Arg
+        | T.UpVar n => E.UpVar n
+        | T.Call f a => E.Call (go f) (go a)
+        | T.Constr tag args => E.Constr tag (go_list args)
+        | T.ElimN n cases target =>
+                let num_upvars := S (T.num_upvars_list_pair cases) in
+                let func := E.Close (base + n) (upvar_list num_upvars) in
+                E.Call func (go target)
+        | T.Close fname free => E.Close fname (go_list free)
+        end in go.
+
+Definition compile_list base :=
+    let go := compile base in
+    let fix go_list es :=
+        match es with
+        | [] => []
+        | e :: es => go e :: go_list es
+        end in go_list.
+
+Ltac refold_compile base :=
+    fold (compile_list base) in *.
+
+Definition compile_pair base :=
+    let go := compile base in
+    let fix go_pair (p : T.expr * T.rec_info) :=
+        let '(e, r) := p in
+        (go e, r) in go_pair.
+
+Definition compile_list_pair base :=
+    let go_pair := compile_pair base in
+    let fix go_list_pair es :=
+        match es with
+        | [] => []
+        | e :: es => go_pair e :: go_list_pair es
+        end in go_list_pair.
+
 
 Definition rec_free :=
     let fix go acc n :=
@@ -24,10 +70,6 @@ Definition rec_free :=
         | 0 => acc
         | S n' => go (E.UpVar n' :: acc) n'
         end in go [].
-
-
-Section compile.
-Open Scope state_monad.
 
 Definition shift : E.expr -> E.expr :=
     let fix go e :=
@@ -52,6 +94,14 @@ Definition shift : E.expr -> E.expr :=
         | E.Close fname free => E.Close fname (go_list free)
         end in go.
 
+Definition shift_list :=
+    let go := shift in
+    let fix go_list es :=
+        match es with
+        | [] => []
+        | e :: es => go e :: go_list es
+        end in go_list.
+
 Definition shift_pair : (E.expr * E.rec_info) -> (E.expr * E.rec_info) :=
     let go := shift in
     let fix go_pair p :=
@@ -65,9 +115,388 @@ Definition shift_list_pair :=
         | p :: ps => go_pair p :: go_list_pair ps
         end in go_list_pair.
 
-Definition get_next_fname base : compiler_monad E.function_name :=
-    fun s => (base + length s, s).
-Definition emit x : compiler_monad unit := fun s => (tt, s ++ [x]).
+Definition compile_eliminator base n cases :=
+    let num_upvars := S (T.num_upvars_list_pair cases) in
+    let cases' := compile_list_pair base cases in
+    let cases'' := shift_list_pair cases' in
+    let rec := E.Close (base + n) (rec_free num_upvars) in
+    E.ElimBody rec cases'' E.Arg.
+
+Fixpoint compile_eliminator_list' base n elims :=
+    match elims with
+    | [] => []
+    | elim :: elims =>
+            compile_eliminator base n elim ::
+            compile_eliminator_list' base (S n) elims
+    end.
+
+Definition compile_eliminator_list base elims :=
+    compile_eliminator_list' base 0 elims.
+
+Definition compile_env elims es :=
+    compile_list (length es) es ++
+    compile_eliminator_list (length es) elims.
+
+
+Section test.
+
+Open Scope state_monad.
+
+Require Tagged TaggedNumberedComp.
+Definition numbered :=
+    (@pair _ _ <$> TaggedNumberedComp.compile Tagged.add_reflect
+               <*> TaggedNumberedComp.compile_list Tagged.add_env) [].
+
+Definition elimfunc :=
+    let '(main, env, elims) := numbered in
+    (compile (length env) main, compile_env elims env).
+
+Eval compute in elimfunc.
+
+Lemma elimfunc_ok : elimfunc = (E.add_reflect, E.add_env).
+reflexivity.
+Qed.
+
+Theorem T_add_2_3 : { x | T.star T.add_env
+        (T.Call (T.Call T.add_reflect (T.nat_reflect 2)) (T.nat_reflect 3)) x }.
+eexists.
+
+unfold T.add_reflect.
+eright. eapply T.CallL, T.MakeCall; try solve [repeat econstructor].
+
+eright. eapply T.MakeCall; try solve [repeat econstructor].
+eright. eapply T.CallL, T.Eliminate; try solve [repeat econstructor]. cbv beta.
+(*
+          (T.ElimN  0
+                [(T.Close  T.elim_zero_lam_b  [T.nat_reflect  3;  T.nat_reflect  2],  []);
+                (T.Close  T.elim_succ_lam_a  [T.nat_reflect  3;  T.nat_reflect  2],
+                [true])]  (T.nat_reflect  2))  (T.nat_reflect  3))  
+                *)
+
+eright. eapply T.CallL, T.CallL, T.MakeCall; try solve [repeat econstructor].
+eright. eapply T.CallL, T.CallR, T.Eliminate; try solve [repeat econstructor]. cbv beta.
+
+eright. eapply T.CallL, T.CallR, T.CallL, T.MakeCall; try solve [repeat econstructor].
+eright. eapply T.CallL, T.CallR, T.CallR, T.Eliminate; try solve [repeat econstructor]. cbv beta.
+
+eright. eapply T.CallL, T.CallR, T.MakeCall; try solve [repeat econstructor].
+eright. eapply T.CallL, T.MakeCall; try solve [repeat econstructor].
+eright. eapply T.MakeCall; try solve [repeat econstructor].
+eright. eapply T.MakeCall; try solve [repeat econstructor].
+eright. eapply T.MakeCall; try solve [repeat econstructor].
+eleft.
+Defined.
+Eval compute in proj1_sig T_add_2_3.
+
+Theorem E_add_2_3 : { x | E.star E.add_env
+        (E.Call (E.Call E.add_reflect (E.nat_reflect 2)) (E.nat_reflect 3)) x }.
+eexists.
+
+unfold E.add_reflect.
+eright. eapply E.CallL, E.MakeCall; try solve [repeat econstructor].
+
+eright. eapply E.MakeCall; try solve [repeat econstructor].
+eright. eapply E.CallL, E.MakeCall; try solve [repeat econstructor].
+eright. eapply E.CallL, E.Eliminate; try solve [repeat econstructor].
+(*
+          (E.ElimBody  (E.Close  E.nat_elim  [E.nat_reflect  3;  E.nat_reflect  2])
+                [(E.Close  E.elim_zero_lam_b  [E.nat_reflect  3;  E.nat_reflect  2],  []);
+                (E.Close  E.elim_succ_lam_a  [E.nat_reflect  3;  E.nat_reflect  2],
+                [true])]  (E.nat_reflect  2))  (E.nat_reflect  3))  
+                *)
+
+eright. eapply E.CallL, E.CallL, E.MakeCall; try solve [repeat econstructor].
+eright. eapply E.CallL, E.CallR, E.MakeCall; try solve [repeat econstructor].
+eright. eapply E.CallL, E.CallR, E.Eliminate; try solve [repeat econstructor].
+
+eright. eapply E.CallL, E.CallR, E.CallL, E.MakeCall; try solve [repeat econstructor].
+eright. eapply E.CallL, E.CallR, E.CallR, E.MakeCall; try solve [repeat econstructor].
+eright. eapply E.CallL, E.CallR, E.CallR, E.Eliminate; try solve [repeat econstructor].
+
+eright. eapply E.CallL, E.CallR, E.MakeCall; try solve [repeat econstructor].
+eright. eapply E.CallL, E.MakeCall; try solve [repeat econstructor].
+eright. eapply E.MakeCall; try solve [repeat econstructor].
+eright. eapply E.MakeCall; try solve [repeat econstructor].
+eright. eapply E.MakeCall; try solve [repeat econstructor].
+eleft.
+Defined.
+Eval compute in proj1_sig E_add_2_3.
+
+End test.
+
+
+Definition env_ok TE EE ELIMS :=
+    EE = compile_env ELIMS TE.
+
+Inductive I_expr (TE : T.env) (EE : E.env) : T.expr -> E.expr -> Prop :=
+| IArg : I_expr TE EE T.Arg E.Arg
+| IUpVar : forall n, I_expr TE EE (T.UpVar n) (E.UpVar n)
+| ICall : forall tf ta ef ea,
+        I_expr TE EE tf ef ->
+        I_expr TE EE ta ea ->
+        I_expr TE EE (T.Call tf ta) (E.Call ef ea)
+| IConstr : forall tag targs eargs,
+        Forall2 (I_expr TE EE) targs eargs ->
+        I_expr TE EE (T.Constr tag targs) (E.Constr tag eargs)
+| IClose : forall fname tfree efree,
+        Forall2 (I_expr TE EE) tfree efree ->
+        I_expr TE EE (T.Close fname tfree) (E.Close fname efree)
+            (* TODO ??? *)
+| IElimN : forall tnum tcases ttarget fname efree etarget erec ecases,
+        fname = length TE + tnum ->
+        nth_error EE fname = Some (E.ElimBody erec ecases E.Arg) ->
+        erec = E.Close fname (rec_free (length efree)) ->
+        ecases = shift_list_pair (compile_list_pair (length TE) tcases) ->
+        I_expr TE EE ttarget etarget ->
+        I_expr TE EE (T.ElimN tnum tcases ttarget)
+                (E.Call (E.Close fname efree) etarget).
+
+Inductive I (TE : T.env) (EE : E.env) : T.state -> E.state -> Prop :=
+| IRun : forall te tl tk ee el ek,
+        I_expr TE EE te ee ->
+        Forall2 (I_expr TE EE) tl el ->
+        (forall tv ev, I_expr TE EE tv ev -> I TE EE (tk tv) (ek ev)) ->
+        I TE EE (T.Run te tl tk) (E.Run ee el ek)
+| IStop : forall te ee,
+        I_expr TE EE te ee ->
+        I TE EE (T.Stop te) (E.Stop ee).
+
+
+
+Lemma compile_list_Forall : forall base tes ees,
+    compile_list base tes = ees <-> Forall2 (fun te ee => compile base te = ee) tes ees.
+induction tes; intros; split; intro HH.
+- simpl in HH. subst. constructor.
+- invc HH. reflexivity.
+- simpl in HH. destruct ees; invc HH. constructor; eauto.
+  rewrite <- IHtes. reflexivity.
+- invc HH. simpl. f_equal.
+  rewrite IHtes. assumption.
+Qed.
+
+Lemma compile_list_Forall' : forall base tes ees,
+    ees = compile_list base tes <-> Forall2 (fun te ee => compile base te = ee) tes ees.
+intros. rewrite <- compile_list_Forall. split; eauto.
+Qed.
+
+Lemma compile_list_length : forall base tes,
+    length (compile_list base tes) = length tes.
+intros. remember (compile_list base tes) as ees.
+rewrite compile_list_Forall' in *.
+symmetry. eauto using Forall2_length.
+Qed.
+
+Lemma compile_eliminator_list'_nth_error : forall base n elims i elim,
+    nth_error elims i = Some elim ->
+    nth_error (compile_eliminator_list' base n elims) i =
+    Some (compile_eliminator base (n + i) elim).
+first_induction elims; intros0 Hnth.
+{ destruct i; simpl in Hnth; discriminate Hnth. }
+destruct i; simpl in Hnth.
+- inject_some. simpl. replace (n + 0) with n by omega. reflexivity.
+- simpl. rewrite IHelims with (1 := **).
+  replace (S n + i) with (n + S i) by omega. reflexivity.
+Qed.
+
+Lemma compile_eliminator_list_nth_error : forall base elims i elim,
+    nth_error elims i = Some elim ->
+    nth_error (compile_eliminator_list base elims) i =
+    Some (compile_eliminator base i elim).
+intros. unfold compile_eliminator_list.
+eapply compile_eliminator_list'_nth_error. assumption.
+Qed.
+
+Lemma compile_eliminator_list'_length : forall base n elims,
+    length (compile_eliminator_list' base n elims) = length elims.
+first_induction elims; intros; simpl.
+- reflexivity.
+- rewrite IHelims. reflexivity.
+Qed.
+
+Lemma compile_eliminator_list_length : forall base elims,
+    length (compile_eliminator_list base elims) = length elims.
+intros. eapply compile_eliminator_list'_length.
+Qed.
+
+
+Lemma env_ok_nth_error : forall TE EE ELIMS i x,
+    env_ok TE EE ELIMS ->
+    nth_error EE (length TE + i) = Some x ->
+    exists cases,
+        nth_error ELIMS i = Some cases /\
+        x = compile_eliminator (length TE) i cases.
+unfold env_ok, compile_env.
+intros0 Henv Hnth.
+
+assert (length EE = length TE + length ELIMS). {
+  subst EE.
+  rewrite app_length, compile_list_length, compile_eliminator_list_length.
+  reflexivity.
+}
+assert (length TE + i < length EE). {
+  rewrite <- nth_error_Some. congruence.
+}
+assert (i < length ELIMS) by omega.
+assert (HH : exists cases, nth_error ELIMS i = Some cases). {
+  on (i < length _), fun H => rename H into HH.
+  rewrite <- nth_error_Some in HH.
+  destruct (nth_error ELIMS i); try congruence.
+  eauto.
+}
+destruct HH as [cases ?].
+exists cases. split; eauto.
+
+fwd eapply compile_eliminator_list_nth_error with (base := length TE); eauto.
+match type of Henv with | EE = ?a ++ ?b =>
+        remember a as EE1; remember b as EE2 end.
+subst EE.
+replace (length TE) with (length EE1) in * by (subst EE1; eauto using compile_list_length).
+erewrite nth_error_app2 in Hnth by omega.
+replace (_ + i - _) with i in * by omega.
+congruence.
+Qed.
+
+Lemma I_expr_value : forall TE EE t e,
+    I_expr TE EE t e ->
+    T.value t ->
+    E.value e.
+induction t using T.expr_ind''; intros0 II Tval; invc II; invc Tval.
+- constructor. list_magic_on (args, (eargs, tt)).
+- constructor. list_magic_on (free, (efree, tt)).
+Qed.
+
+Lemma I_expr_value' : forall TE EE t e,
+    I_expr TE EE t e ->
+    E.value e ->
+    T.value t.
+make_first e.
+induction e using E.expr_ind''; intros0 II Eval; invc II; invc Eval.
+- constructor. list_magic_on (args, (targs, tt)).
+- constructor. list_magic_on (free, (tfree, tt)).
+Qed.
+
+(*
+Lemma I_num_upvars : forall TE EE t e,
+    I TE EE t e ->
+    E.num_upvars e <= T.num_upvars t.
+intros TE EE.
+induction t using T.expr_rect_mut with
+    (Pl := fun ts => forall es,
+        Forall2 (I TE EE) ts es ->
+        E.num_upvars_list es <= T.num_upvars_list ts)
+    (Pp := fun tp => forall ep,
+        I TE EE (fst tp) (fst ep) ->
+        E.num_upvars_pair ep <= T.num_upvars_pair tp)
+    (Plp := fun tps => forall eps,
+        Forall2 (fun tp ep => I TE EE (fst tp) (fst ep)) tps eps ->
+        E.num_upvars_list_pair eps <= T.num_upvars_list_pair tps);
+intros0 II;
+try match goal with | [ |- E.num_upvars _ <= _ ] => invc II end;
+simpl; T.refold_num_upvars; E.refold_num_upvars.
+
+- lia.
+- lia.
+- specialize (IHt1 ?? ** ).
+  specialize (IHt2 ?? ** ).
+  lia.
+- specialize (IHt ?? ** ).
+  assumption.
+- admit.
+- specialize (IHt ?? ** ).
+  assumption.
+
+- invc II. simpl. lia.
+- invc II. simpl.
+  specialize (IHt ?? ** ).
+  specialize (IHt0 ?? ** ).
+  lia.
+
+- destruct ep. simpl. eauto.
+
+- invc II. simpl. lia.
+- invc II. simpl.
+  specialize (IHt ?? ** ).
+  specialize (IHt0 ?? ** ).
+  lia.
+Admitted.
+*)
+
+(*
+
+Lemma I_closed : forall TE EE t e,
+    I TE EE t e ->
+    T.closed t ->
+    E.closed e.
+induction t using T.expr_ind''; intros0 II Tcls; invc II; invc Tcls.
+- constructor; eauto.
+- constructor. list_magic_on (args, (eargs, tt)).
+- constructor; eauto. constructor.
+*)
+
+Theorem I_sim : forall TE EE ELIMS t t' e,
+    env_ok TE EE ELIMS ->
+    I TE EE t e ->
+    T.sstep TE t t' ->
+    exists e',
+        E.splus EE e e' /\
+        I TE EE t' e'.
+destruct t as [te tl tk | te]; cycle 1.
+  { intros0 Henv II Tstep. invc Tstep. }
+generalize dependent tk. generalize dependent tl.
+induction te using T.expr_ind''; intros0 Henv II Tstep;
+invc Tstep; invc II; try on (I_expr _ _ _ _), invc;
+simpl in *; refold_compile (length TE).
+
+- break_match; try discriminate. inject_some.
+  on (Forall2 _ _ _), invc.
+
+  eexists. split. eapply E.SPlusOne, E.SArg.
+  + reflexivity.
+  + eauto.
+
+- break_match; try discriminate. 
+  on (Forall2 _ _ _), invc.
+  fwd eapply length_nth_error_Some.
+    { eapply Forall2_length. eassumption. }
+    { eassumption. }
+  break_exists.
+
+  eexists. split. eapply E.SPlusOne, E.SUpVar.
+  + simpl. eassumption.
+  + fwd eapply Forall2_nth_error; try eassumption. eauto.
+
+- admit.
+
+- admit.
+
+- on (I_expr _ _ (T.Close _ _) _), invc.
+  eexists. split. eapply E.SPlusOne, E.SMakeCall.
+  + list_magic_on (free, (efree, tt)). eauto using I_expr_value.
+  + eauto using I_expr_value.
+  + admit. (* fname valid in TE -> fname valid in EE *)
+  + constructor; eauto.
+    admit. (* I_expr body ebody *)
+
+- admit.
+
+- admit.
+
+- eexists. split. eapply E.SPlusOne, E.SCallR.
+  + admit. (* need to compute all `efree` to values *)
+  + firstorder eauto using I_expr_value'.
+  + constructor; eauto.
+    intros. constructor; eauto.
+    econstructor; eauto.
+
+- admit.
+
+- admit.
+
+- admit.
+
+Admitted.
+
+(*
 
 Definition gen_eliminator base cases : compiler_monad (E.function_name * nat) :=
     let cases' := shift_list_pair cases in
@@ -137,3 +566,4 @@ Lemma compile_test : compile_program (T.add_reflect, T.add_env) = (E.add_reflect
 reflexivity.
 Qed.
 
+*)
